Handle pattern-matching in cf.
Some simple (hopefully) cheats are remaining, but otherwise the
soundness proof has been updated.

characteristic/cfScript.sml
@@ -3,6 +3,7 @@ open set_sepTheory helperLib ml_translatorTheory
 open semanticPrimitivesTheory ConseqConv
 open cfHeapsBaseTheory cfHeapsTheory cfHeapsBaseLib cfStoreTheory
 open cfNormalizeTheory cfAppTheory
+open patternMatchesTheory
 
 val _ = new_theory "cf"
 
@@ -18,6 +19,8 @@ fun rpt_drule_then thm_tac thm =
 fun progress thm = rpt_drule_then strip_assume_tac thm
 
 fun sing x = [x]
+
+fun try_finally tac = TRY (tac \\ NO_TAC)
 
 (*------------------------------------------------------------------*)
 (* Machinery for dealing with n-ary applications/functions in cf.
@@ -328,19 +331,29 @@ val letrec_pull_params_repack = store_thm ("letrec_pull_params_repack",
 (** Extending environments *)
 
 (* [extend_env] *)
-val extend_env_def = Define `
-  extend_env [] [] env = env /\
-  extend_env (n::ns) (xv::xvs) env =
-    extend_env ns xvs (env with v := (n,xv)::env.v)`
+val extend_env_v_def = Define `
+  extend_env_v [] [] env_v = env_v /\
+  extend_env_v (n::ns) (xv::xvs) env_v =
+    extend_env_v ns xvs ((n,xv)::env_v)`
 
-val extend_env_rcons = store_thm ("extend_env_rcons",
-  ``!ns xvs n xv env.
+val extend_env_def = Define `
+  extend_env ns xvs env = (env with v := extend_env_v ns xvs env.v)`
+
+val extend_env_v_rcons = store_thm ("extend_env_v_rcons",
+  ``!ns xvs n xv env_v.
      LENGTH ns = LENGTH xvs ==>
-     extend_env (ns ++ [n]) (xvs ++ [xv]) env =
-     let env' = extend_env ns xvs env in
-     (env' with v := (n,xv) :: env'.v)``,
+     extend_env_v (ns ++ [n]) (xvs ++ [xv]) env_v =
+     (n,xv) :: extend_env_v ns xvs env_v``,
   Induct \\ rpt strip_tac \\ first_assum (assume_tac o GSYM) \\
-  fs [LENGTH_NIL, LENGTH_CONS, extend_env_def]
+  fs [LENGTH_NIL, LENGTH_CONS, extend_env_v_def]
+)
+
+val extend_env_v_zip = store_thm ("extend_env_v_zip",
+  ``!ns xvs env_v.
+    LENGTH ns = LENGTH xvs ==>
+    extend_env_v ns xvs env_v = ZIP (REVERSE ns, REVERSE xvs) ++ env_v``,
+  Induct \\ rpt strip_tac \\ first_assum (assume_tac o GSYM) \\
+  fs [LENGTH_NIL, LENGTH_CONS, extend_env_v_def, GSYM ZIP_APPEND]
 )
 
 (* [build_rec_env_aux] *)
@@ -372,18 +385,518 @@ val build_rec_env_zip = store_thm ("build_rec_env_zip",
 )
 
 (* [extend_env_rec] *)
+val extend_env_v_rec_def = Define `
+  extend_env_v_rec rec_ns rec_xvs ns xvs env_v =
+    extend_env_v ns xvs (ZIP (rec_ns, rec_xvs) ++ env_v)`
+
 val extend_env_rec_def = Define `
   extend_env_rec rec_ns rec_xvs ns xvs env =
-    extend_env ns xvs (env with v := ZIP (rec_ns, rec_xvs) ++ env.v)`
+    env with v := extend_env_v_rec rec_ns rec_xvs ns xvs env.v`
 
 val extend_env_rec_build_rec_env = store_thm ("extend_env_rec_build_rec_env",
-  ``!funs env.
-     extend_env_rec
+  ``!funs env env_v.
+     extend_env_v_rec
        (MAP (\ (f,_,_). f) funs)
        (MAP (\ (f,_,_). naryRecclosure env (letrec_pull_params funs) f) funs)
-       [] [] env =
-     (env with v := build_rec_env funs env env.v)``,
-  rpt strip_tac \\ fs [extend_env_rec_def, extend_env_def, build_rec_env_zip]
+       [] [] env_v =
+     build_rec_env funs env env_v``,
+  rpt strip_tac \\ fs [extend_env_v_rec_def, extend_env_v_def, build_rec_env_zip]
+)
+
+(*------------------------------------------------------------------*)
+(** Pattern matching.
+
+    CakeML pattern-matching is translated to pattern-matching in HOL
+    using the src/pattern_matching library, by Tuerk et al.
+
+    Restrictions:
+    - the CakeML pattern-matching must "typecheck" (does not raise
+      Match_type_error)
+    - patterns that use [Pref] are not currently supported
+*)
+
+(* [v_of_pat]: from a pattern and a list of instantiations for the pattern
+   variables, produce a semantic value
+*)
+
+val v_of_matching_pat_aux_measure_def = Define `
+  v_of_matching_pat_aux_measure x =
+    sum_CASE x
+      (\(_,p,_). pat_size p)
+      (\(_,ps,_). list_size pat_size ps)`
+
+val v_of_pat_def = tDefine "v_of_pat" `
+  v_of_pat envC (Pvar x) insts =
+    (case insts of
+         xv::rest => SOME (xv, rest)
+       | _ => NONE) /\
+  v_of_pat envC (Plit l) insts = SOME (Litv l, insts) /\
+  v_of_pat envC (Pcon c args) insts =
+    (case v_of_pat_list envC args insts of
+         SOME (argsv, insts_rest) =>
+         (case c of
+              NONE => SOME (Conv NONE argsv, insts_rest)
+            | SOME id =>
+              case lookup_alist_mod_env id envC of
+                  NONE => NONE
+                | SOME (len, t) =>
+                  if len = LENGTH argsv then
+                    SOME (Conv (SOME (id_to_n id,t)) argsv, insts_rest)
+                  else NONE)
+      | NONE => NONE) /\
+  v_of_pat _ (Pref pat) _ =
+    NONE (* unsupported *) /\
+  v_of_pat _ _ _ = NONE /\
+
+  v_of_pat_list _ [] insts = SOME ([], insts) /\
+  v_of_pat_list envC (p::argspat) insts =
+    (case v_of_pat envC p insts of
+         SOME (v, insts_rest) =>
+         (case v_of_pat_list envC argspat insts_rest of
+              SOME (vs, insts_rest') => SOME (v::vs, insts_rest')
+            | NONE => NONE)
+       | NONE => NONE) /\
+  v_of_pat_list _ _ _ = NONE`
+
+  (WF_REL_TAC `measure v_of_matching_pat_aux_measure` \\
+   fs [v_of_matching_pat_aux_measure_def, list_size_def,
+       astTheory.pat_size_def] \\
+   gen_tac \\ Induct \\ fs [list_size_def, astTheory.pat_size_def])
+
+val v_of_pat_ind = fetch "-" "v_of_pat_ind"
+
+val v_of_pat_insts_length = store_thm ("v_of_pat_insts_length",
+  ``(!envC pat insts v insts_rest.
+       v_of_pat envC pat insts = SOME (v, insts_rest) ==>
+       (LENGTH insts = LENGTH (pat_bindings pat []) <=> insts_rest = [])) /\
+    (!envC pats insts vs insts_rest.
+       v_of_pat_list envC pats insts = SOME (vs, insts_rest) ==>
+       (LENGTH insts = LENGTH (pats_bindings pats []) <=> insts_rest = []))``,
+  cheat
+)
+
+val v_of_pat_extend_insts = store_thm ("v_of_pat_extend_insts",
+  ``(!envC pat insts v rest insts'.
+       v_of_pat envC pat insts = SOME (v, rest) ==>
+       v_of_pat envC pat (insts ++ insts') = SOME (v, rest ++ insts')) /\
+    (!envC pats insts vs rest insts'.
+       v_of_pat_list envC pats insts = SOME (vs, rest) ==>
+       v_of_pat_list envC pats (insts ++ insts') = SOME (vs, rest ++ insts'))``,
+  cheat
+)
+
+val v_of_pat_remove_rest_insts = store_thm ("v_of_pat_remove_rest_insts",
+  ``(!envC pat insts v rest.
+       v_of_pat envC pat insts = SOME (v, rest) ==>
+       ?insts'.
+         insts = insts' ++ rest /\
+         LENGTH insts' = LENGTH (pat_bindings pat []) /\
+         v_of_pat envC pat insts' = SOME (v, [])) /\
+    (!envC pats insts vs rest.
+       v_of_pat_list envC pats insts = SOME (vs, rest) ==>
+       ?insts'.
+         insts = insts' ++ rest /\
+         LENGTH insts' = LENGTH (pats_bindings pats []) /\
+         v_of_pat_list envC pats insts' = SOME (vs, []))``,
+  cheat
+)
+
+val v_of_pat_list_length = store_thm ("v_of_pat_list_length",
+  ``!envC pats insts vs rest.
+      v_of_pat_list envC pats insts = SOME (vs, rest) ==>
+      LENGTH pats = LENGTH vs``,
+  cheat
+)
+
+val v_of_pat_insts_unique = store_thm ("v_of_pat_insts_unique",
+  ``(!envC pat insts rest v.
+       v_of_pat envC pat insts = SOME (v, rest) ==>
+       (!insts'. v_of_pat envC pat insts' = SOME (v, rest) <=> (insts' = insts))) /\
+    (!envC pats insts rest vs.
+       v_of_pat_list envC pats insts = SOME (vs, rest) ==>
+       (!insts'. v_of_pat_list envC pats insts' = SOME (vs, rest) <=> (insts' = insts)))``,
+
+  HO_MATCH_MP_TAC v_of_pat_ind \\ rpt strip_tac \\
+  try_finally (fs [v_of_pat_def] \\ every_case_tac \\ fs [])
+  THEN1 (
+    fs [v_of_pat_def] \\ every_case_tac \\ fs [] \\ rw [] \\
+    TRY (first_assum (qspec_then `insts'` assume_tac)) \\
+    TRY (strip_tac \\ rw [] \\ fs []) \\
+    TRY (qpat_assum `LENGTH _ = LENGTH _` (K all_tac)) (* otherwise fs[] loops? *) \\
+    TRY (eq_tac \\ strip_tac \\ rw [] \\ fs []) \\ rw []
+  )
+  THEN1 (
+    fs [v_of_pat_def] \\ every_case_tac \\ fs [] \\ rw [] \\
+    TRY (strip_tac \\ rw [] \\ fs []) \\ rw [] \\ fs [] \\
+    eq_tac \\ rw [] \\ fs [] \\ rw [] \\ fs []
+  )
+)
+
+(* [v_of_pat_norest]: Wrapper that checks that there are no remaining
+   instantiations
+*)
+
+val v_of_pat_norest_def = Define `
+  v_of_pat_norest envC pat insts =
+    case v_of_pat envC pat insts of
+        SOME (v, []) => SOME v
+      | _ => NONE`
+
+val v_of_pat_norest_insts_length = store_thm ("v_of_pat_norest_insts_length",
+  ``!envC pat insts v.
+      v_of_pat_norest envC pat insts = SOME v ==>
+      LENGTH insts = LENGTH (pat_bindings pat [])``,
+  rpt strip_tac \\ fs [v_of_pat_norest_def] \\ every_case_tac \\ fs [] \\
+  rw [] \\ progress (fst (CONJ_PAIR v_of_pat_insts_length)) \\ fs []
+)
+
+val v_of_pat_norest_insts_unique = store_thm ("v_of_pat_norest_insts_unique",
+  ``!envC pat insts v.
+      v_of_pat_norest envC pat insts = SOME v ==>
+      (!insts'. v_of_pat_norest envC pat insts' = SOME v <=> (insts' = insts))``,
+  rpt strip_tac \\ fs [v_of_pat_norest_def] \\
+  every_case_tac \\ fs [] \\ rw [] \\ 
+  try_finally (strip_tac \\ rw [] \\ fs []) \\
+  eq_tac \\ rw [] \\ fs [] \\
+  progress (fst (CONJ_PAIR (v_of_pat_insts_unique))) \\ fs []
+)
+
+
+(* Predicates that discriminate the patterns we want to deal
+   with. [validate_pat] packs them all up.
+*)
+
+val pat_typechecks_def = Define `
+  pat_typechecks envC s pat v env =
+    (pmatch envC s pat v env <> Match_type_error)`
+
+val pat_without_Pref_def = tDefine "pat_without_Pref" `
+  pat_without_Pref (Pvar _) = T /\
+  pat_without_Pref (Plit _) = T /\
+  pat_without_Pref (Pcon _ args) =
+    EVERY pat_without_Pref args /\
+  pat_without_Pref (Pref _) = F`
+
+  (WF_REL_TAC `measure pat_size` \\
+   Cases \\ Induct \\ fs [basicSizeTheory.option_size_def] \\
+   fs [list_size_def, astTheory.pat_size_def] \\ rpt strip_tac \\ fs [] \\
+   first_assum progress \\ fs [])
+
+val validate_pat_def = Define `
+  validate_pat envC s pat v env =
+    (pat_typechecks envC s pat v env /\
+     pat_without_Pref pat /\
+     ALL_DISTINCT (pat_bindings pat []))`
+
+
+(* [PMATCH_ROW_of_pat]: the instance of [PMATCH_ROW] that corresponds to a
+   CakeML pattern
+*)
+
+val PMATCH_ROW_of_pat_def = Define `
+  PMATCH_ROW_of_pat pat branch_cf env =
+    PMATCH_ROW
+      (\insts. v_of_pat_norest env.c pat insts)
+      (\_. T)
+      (\insts.
+         \env. branch_cf (extend_env (REVERSE (pat_bindings pat [])) insts env))`
+
+
+(* Lemmas that relate [v_of_pat] and [pmatch], the pattern-matching function
+   from the semantics.
+*)
+
+val pat_bindings_def = astTheory.pat_bindings_def
+val pmatch_def = terminationTheory.pmatch_def
+val pmatch_ind = terminationTheory.pmatch_ind
+
+val pmatch_list_match_length = store_thm ("pmatch_list_match_length",
+  ``!envC s pats args env env'.
+     pmatch_list envC s pats args env = Match env' ==>
+     LENGTH pats = LENGTH args``,
+  Induct_on `pats` \\ Cases_on `args` \\ fs [pmatch_def] \\
+  rpt strip_tac \\ every_case_tac \\ fs [] \\ first_assum irule \\ instantiate
+)
+
+val v_of_pat_pmatch = store_thm ("v_of_pat_pmatch",
+  ``(!envC s pat v env_v insts.
+      v_of_pat envC pat insts = SOME (v, []) ==>
+      pmatch envC s pat v env_v = Match
+        (ZIP (pat_bindings pat [], REVERSE insts) ++ env_v)) /\
+    (!envC s pats vs env_v insts.
+      v_of_pat_list envC pats insts = SOME (vs, []) ==>
+      pmatch_list envC s pats vs env_v = Match
+        (ZIP (pats_bindings pats [], REVERSE insts) ++ env_v))``,
+
+  HO_MATCH_MP_TAC pmatch_ind \\ rpt strip_tac \\ rw [] \\
+  try_finally (
+    fs [pmatch_def, v_of_pat_def, pat_bindings_def] \\
+    every_case_tac \\ fs [] \\
+    every_case_tac \\ fs []
+  )
+  THEN1 (
+    fs [pmatch_def, v_of_pat_def, pat_bindings_def] \\
+    every_case_tac \\ fs [] \\ rw []
+    THEN1 (progress v_of_pat_list_length \\ fs []) \\
+    `!(n:tvarN) t. same_ctor (n, t) (n, t)` by (
+      Cases_on `n` \\ Cases_on `t` \\ fs [same_ctor_def]
+    ) \\ fs []
+  )
+  THEN1 (
+    fs [pmatch_def, v_of_pat_def, pat_bindings_def] \\
+    every_case_tac \\ fs [] \\ rw [] \\
+    progress v_of_pat_list_length \\ fs []
+  )
+  THEN1 (
+    fs [pmatch_def, pat_bindings_def, v_of_pat_def] \\
+    every_case_tac \\ fs [] \\ rw [] \\
+    try_finally (
+      progress (fst (CONJ_PAIR v_of_pat_remove_rest_insts)) \\ rw [] \\
+      rename1 `insts' ++ rest` \\ first_assum (qspec_then `insts'` (fs o sing))
+    ) \\
+    once_rewrite_tac [snd (CONJ_PAIR evalPropsTheory.pat_bindings_accum)] \\
+    fs [] \\ progress (fst (CONJ_PAIR v_of_pat_remove_rest_insts)) \\ rw [] \\
+    fs [REVERSE_APPEND] \\ progress (snd (CONJ_PAIR v_of_pat_insts_length)) \\
+    fs [GSYM ZIP_APPEND] \\ once_rewrite_tac [GSYM APPEND_ASSOC] \\
+    rpt (first_x_assum progress) \\ rw []
+  )
+)
+
+val v_of_pat_norest_pmatch = store_thm ("v_of_pat_norest_pmatch",
+  ``!envC s pat v env_v insts.
+     v_of_pat_norest envC pat insts = SOME v ==>
+     pmatch envC s pat v env_v = Match
+       (ZIP (pat_bindings pat [], REVERSE insts) ++ env_v)``,
+  rpt strip_tac \\ fs [v_of_pat_norest_def] \\
+  every_case_tac \\ fs [v_of_pat_pmatch]
+)
+
+val pmatch_v_of_pat = store_thm ("pmatch_v_of_pat",
+  ``(!envC s pat v env_v env_v'.
+      pmatch envC s pat v env_v = Match env_v' ==>
+      pat_without_Pref pat ==>
+      ?insts.
+        env_v' = ZIP (pat_bindings pat [], REVERSE insts) ++ env_v /\
+        v_of_pat envC pat insts = SOME (v, [])) /\
+    (!envC s pats vs env_v env_v'.
+      pmatch_list envC s pats vs env_v = Match env_v' ==>
+      EVERY (\pat. pat_without_Pref pat) pats ==>
+      ?insts.
+        env_v' = ZIP (pats_bindings pats [], REVERSE insts) ++ env_v /\
+        v_of_pat_list envC pats insts = SOME (vs, []))``,
+
+  HO_MATCH_MP_TAC pmatch_ind \\ rpt strip_tac \\ rw [] \\
+  try_finally (fs [pmatch_def, v_of_pat_def, pat_bindings_def])
+  THEN1 (
+    fs [pmatch_def, v_of_pat_def, pat_bindings_def] \\
+    qpat_assum `_ = _` (fs o sing o GSYM) \\
+    rename1 `[(x,xv)]` \\ qexists_tac `[xv]` \\ fs []
+  )
+  THEN1 (
+    fs [pmatch_def, v_of_pat_def, pat_bindings_def] \\
+    every_case_tac \\ fs []
+  )
+  THEN1 (
+    fs [pmatch_def, pat_without_Pref_def] \\ every_case_tac \\ fs [] \\
+    fs [pat_bindings_def] \\ qexists_tac `insts` \\ fs [] \\
+    rename1 `same_ctor (id_to_n id1, t1) (n2, t2)` \\
+    `t1 = t2 /\ id_to_n id1 = n2` by
+      (irule evalPropsTheory.same_ctor_and_same_tid \\ fs []) \\ rw [] \\
+    rewrite_tac [v_of_pat_def] \\ fs [] \\ progress v_of_pat_list_length
+  )
+  THEN1 (
+    fs [pmatch_def, pat_without_Pref_def] \\ every_case_tac \\ fs [] \\
+    fs [pat_bindings_def] \\ qexists_tac `insts` \\ fs [] \\
+    rewrite_tac [v_of_pat_def] \\ every_case_tac \\ fs []
+  )
+  THEN1 (fs [pat_without_Pref_def])
+  THEN1 (
+    fs [pmatch_def] \\ every_case_tac \\ fs [] \\ rw [] \\
+    first_assum progress \\ rw [] \\ fs [pat_bindings_def] \\
+    once_rewrite_tac [evalPropsTheory.pat_bindings_accum] \\ fs [] \\
+    rename1 `ZIP (pat_bindings pat [], REVERSE insts)` \\
+    rename1 `ZIP (pats_bindings pats [], REVERSE insts')` \\
+    qexists_tac `insts ++ insts'` \\
+    progress (fst (CONJ_PAIR v_of_pat_insts_length)) \\
+    progress (snd (CONJ_PAIR v_of_pat_insts_length)) \\ fs [ZIP_APPEND] \\
+    rpt_drule_then (qspec_then `insts'` assume_tac)
+      (fst (CONJ_PAIR v_of_pat_extend_insts)) \\
+    rpt_drule_then (qspec_then `insts'` assume_tac)
+      (snd (CONJ_PAIR v_of_pat_extend_insts)) \\
+    fs [v_of_pat_def]
+  )
+)
+
+val pmatch_v_of_pat_norest = store_thm ("pmatch_v_of_pat_norest",
+  ``!envC s pat v env_v env_v'.
+      pmatch envC s pat v env_v = Match env_v' ==>
+      pat_without_Pref pat ==>
+      ?insts.
+        env_v' = ZIP (pat_bindings pat [], REVERSE insts) ++ env_v /\
+        v_of_pat_norest envC pat insts = SOME v``,
+  rpt strip_tac \\ progress (fst (CONJ_PAIR pmatch_v_of_pat)) \\ fs [] \\
+  qexists_tac `insts` \\ fs [v_of_pat_norest_def]
+)
+
+val v_of_pat_Con_cons = Q.prove (
+  `!envC env_v s pat v env_v' pats vs insts insts'.
+     pmatch envC s pat v env_v = Match env_v' ==>
+     pat_without_Pref pat ==>
+     v_of_pat envC (Pcon NONE pats) insts' = SOME (Conv NONE vs, []) ==>
+     ?insts.
+       env_v' = ZIP (pat_bindings pat [], REVERSE insts) ++ env_v /\
+       v_of_pat envC (Pcon NONE (pat::pats)) (insts ++ insts') = SOME (Conv NONE (v::vs), [])`,
+
+  rpt strip_tac \\ progress (fst (CONJ_PAIR pmatch_v_of_pat)) \\ rw [] \\
+  rename1 `ZIP (pat_bindings pat [], REVERSE insts)` \\ qexists_tac `insts` \\
+  rpt_drule_then (qspec_then `insts'` assume_tac)
+    (fst (CONJ_PAIR v_of_pat_extend_insts)) \\ fs [] \\
+  qpat_assum `v_of_pat _ (Pcon _ pats) _ = _`
+    (assume_tac o SIMP_RULE std_ss [v_of_pat_def]) \\ every_case_tac \\ rw [] \\
+  fs [build_conv_def] \\ rw [] \\
+  rpt_drule_then (qspec_then `insts'` assume_tac)
+    (snd (CONJ_PAIR v_of_pat_extend_insts)) \\ fs [] \\
+  rewrite_tac [v_of_pat_def] \\ every_case_tac \\ fs [] \\ rw []
+)
+
+
+(* Lemmas relating our [PMATCH_ROW]s with the semantic pattern-matching [pmatch]
+*)
+
+val PMATCH_ROW_pmatch = store_thm ("PMATCH_ROW_pmatch",
+  ``!pat bcf s env v cf H Q.
+     PMATCH_ROW_of_pat pat bcf env (SOME v) = SOME cf ==>
+     cf env H Q ==>
+     ?env_v'.
+       pmatch env.c s pat v env.v = Match env_v' /\
+       bcf (env with v := env_v') H Q``,
+
+  rpt strip_tac \\
+  fs [PMATCH_ROW_of_pat_def, PMATCH_ROW_def, PMATCH_ROW_COND_def, some_def] \\
+  rw [] \\ fs [] \\
+  progress v_of_pat_norest_insts_length \\
+  rpt_drule_then (qspecl_then [`s`, `env.v`] assume_tac) v_of_pat_norest_pmatch \\
+  instantiate \\ progress v_of_pat_norest_insts_unique \\ fs [SELECT_UNIQUE] \\
+  fs [extend_env_def, extend_env_v_zip] 
+)
+
+val PMATCH_ROW_of_pat_matching_Con_NONE = Q.prove (
+  `!env pcname pcnum pctid vcname vcn vctid pats args bcf.
+   lookup_alist_mod_env pcname env.c = SOME (pcnum, pctid) ==>
+   vcname = (vcn, vctid) ==>
+   pctid = vctid /\ id_to_n pcname = vcn ==>
+   LENGTH pats = pcnum ==>
+   PMATCH_ROW_of_pat (Pcon (SOME pcname) pats) bcf env (SOME (Conv (SOME vcname) args)) = NONE ==>
+   PMATCH_ROW_of_pat (Pcon NONE pats) bcf env (SOME (Conv NONE args)) = NONE`,
+
+  rpt strip_tac \\
+  fs [PMATCH_ROW_of_pat_def, PMATCH_ROW_def, PMATCH_ROW_COND_def, some_def] \\
+  qx_gen_tac `inst` \\ pop_assum (qspec_then `inst` assume_tac) \\ rw [] \\
+  fs [v_of_pat_norest_def] \\ every_case_tac \\ fs [] \\
+  fs [v_of_pat_def] \\ every_case_tac \\ fs [] \\ rw [] \\
+  progress v_of_pat_list_length
+)
+
+val PMATCH_ROW_of_pat_con_cons_NONE = Q.prove (
+  `!env s pat v env_v' pats args bcf.
+     pmatch env.c s pat v env.v = Match env_v' ==>
+     pat_without_Pref pat ==>
+     PMATCH_ROW_of_pat (Pcon NONE (pat::pats)) bcf env
+       (SOME (Conv NONE (v::args))) = NONE ==>
+     PMATCH_ROW_of_pat (Pcon NONE pats) bcf (env with v := env_v')
+       (SOME (Conv NONE args)) = NONE`,
+
+  rpt strip_tac \\
+  fs [PMATCH_ROW_of_pat_def, PMATCH_ROW_def, PMATCH_ROW_COND_def, some_def] \\
+  qx_gen_tac `insts` \\ rewrite_tac [v_of_pat_norest_def] \\
+  every_case_tac \\ fs [] \\ strip_tac \\ first_x_assum irule \\ rw [] \\
+  progress v_of_pat_Con_cons \\ rw [] \\
+  rename1 `v_of_pat _ (Pcon _ (_::_)) (insts_pat ++ insts_pats)` \\
+  qexists_tac `insts_pat ++ insts_pats` \\ 
+  fs [v_of_pat_norest_def] \\ every_case_tac \\ fs []
+)
+
+val PMATCH_ROW_pmatch_nomatch = store_thm ("PMATCH_ROW_pmatch_nomatch",
+  ``(!pat env s v (branch_cf: v environment -> 'a).
+      pat_without_Pref pat ==>
+      pmatch env.c s pat v env.v <> Match_type_error ==>
+      PMATCH_ROW_of_pat pat branch_cf env (SOME v) = NONE ==>
+      pmatch env.c s pat v env.v = No_match) /\
+    (!pats env s vs (branch_cf: v environment -> 'a) cname pcname.
+      EVERY (\pat. pat_without_Pref pat) pats ==>
+      pmatch env.c s (Pcon NONE pats) (Conv NONE vs) env.v <> Match_type_error ==>
+      PMATCH_ROW_of_pat (Pcon NONE pats) branch_cf env (SOME (Conv NONE vs)) = NONE ==>
+      pmatch_list env.c s pats vs env.v = No_match)``,
+
+  HO_MATCH_MP_TAC astTheory.pat_induction \\
+  rpt strip_tac
+  THEN1 (
+    fs [PMATCH_ROW_of_pat_def, PMATCH_ROW_def, PMATCH_ROW_COND_def, some_def] \\
+    first_assum (qspec_then `[v]` assume_tac) \\
+    fs [v_of_pat_norest_def, v_of_pat_def]
+  )
+  THEN1 (
+    fs [PMATCH_ROW_of_pat_def, PMATCH_ROW_def, PMATCH_ROW_COND_def, some_def] \\
+    first_x_assum (qspec_then `[]` assume_tac) \\
+    fs [v_of_pat_norest_def, v_of_pat_def] \\ rename1 `Litv l <> v` \\
+    Cases_on `v` \\ fs [pmatch_def] \\ every_case_tac \\ fs []
+  )
+  THEN1 (
+    qpat_assum `pmatch _ _ _ _ _ <> _` mp_tac \\
+    Cases_on `v` \\ try_finally (fs [pmatch_def] \\ every_case_tac) \\
+    rename1 `Conv name_opt args` \\ rename1 `Pcon pname_opt _` \\
+    Cases_on `name_opt` \\ Cases_on `pname_opt` \\ try_finally (fs [pmatch_def])
+    THEN1 (
+      fs [pmatch_def] \\ every_case_tac \\ fs [] \\ strip_tac \\
+      first_assum irule \\ fs [pat_without_Pref_def] \\ instantiate
+    )
+    THEN1 (
+      rename1 `Conv (SOME cname) _` \\ Cases_on `cname` \\
+      fs [pat_without_Pref_def] \\
+      (* At this point:
+         - either the constructors are differents (and in this case, pmatch ... = No_match,
+           which proves the goal)... *)
+      fs [pmatch_def] \\ every_case_tac \\ strip_tac \\
+      (* - or the constructors are the same, and:
+           - pmatch_list ... = No_match, which proves the goal
+           - pmatch_list ... = Match, then we know LENGTH pats = LENGTH args, and
+             modulo additional lemmas we can use the induction hypothesis to prove
+             pmatch_list ... = No_match, proving the goal that became F *)
+      Cases_on `pmatch_list env.c s pats args env.v` \\ fs [] \\ rw [] \\
+      progress pmatch_list_match_length \\
+      `pmatch_list env.c s pats args env.v = No_match` by (
+        first_assum irule
+        THEN1 (every_case_tac \\ fs [])
+        THEN1 (
+          qexists_tac `branch_cf` \\
+          irule PMATCH_ROW_of_pat_matching_Con_NONE \\ instantiate \\
+          rename1 `same_ctor (id_to_n id1, tid1) (n2, tid2)` \\
+          qsuff_tac `tid1 = tid2 /\ id_to_n id1 = n2`
+            THEN1 (fs [CONJ_COMM, EQ_SYM]) \\
+          irule evalPropsTheory.same_ctor_and_same_tid \\ fs []
+        )
+      ) \\ fs []
+    )
+  )
+  THEN1 (
+    fs [pat_without_Pref_def]
+  )
+  THEN1 (
+    Cases_on `vs` \\ fs [pmatch_def] \\
+    fs [PMATCH_ROW_of_pat_def, PMATCH_ROW_def, PMATCH_ROW_COND_def, some_def] \\
+    first_x_assum (qspec_then `[]` assume_tac) \\
+    fs [v_of_pat_norest_def, v_of_pat_def, build_conv_def]
+  )
+  THEN1 (
+    Cases_on `vs` \\ fs [pmatch_def] \\ every_case_tac \\ fs [] \\
+    progress (fst (CONJ_PAIR evalPropsTheory.pmatch_extend)) \\ rw [] \\
+    rename1 `pmatch_list _ _ _ args (matched_env ++ env.v)` \\
+    qsuff_tac `pmatch_list (env with v := matched_env ++ env.v).c s pats args
+                           (env with v := matched_env ++ env.v).v = No_match`
+      THEN1 (fs []) \\
+    first_assum irule \\ fs [] \\ qexists_tac `branch_cf` \\
+    irule PMATCH_ROW_of_pat_con_cons_NONE \\ instantiate
+  )
 )
 
 (*------------------------------------------------------------------*)
@@ -568,6 +1081,16 @@ val cf_aw8update_def = Define `
       exp2v env xw = SOME (Litv (Word8 w)) /\
       app_aw8update l i w H Q)`
 
+val cf_mat_def = Define `
+  cf_mat e pats branches = \env. local (\H Q.
+    ?v branch_cf.
+      exp2v env e = SOME v /\
+      (!s. EVERY (\pat. validate_pat env.c s pat v env.v) pats) /\
+      PMATCH (SOME v) branches = branch_cf /\
+      branch_cf <> PMATCH_INCOMPLETE /\
+      branch_cf env H Q)`
+
+(* todo: replace by THE *)
 val SOME_val_def = Define `
   SOME_val (SOME x) = x`
 
@@ -631,6 +1154,12 @@ val cf_def = tDefine "cf" `
              | [l; n; w] => cf_aw8update l n w
              | _ => cf_bottom)
         | _ => cf_bottom) /\
+  cf (p:'ffi ffi_proj) (Mat e branches) =
+    (\env.
+       cf_mat e
+         (MAP FST branches)
+         (MAP (\b. PMATCH_ROW_of_pat (FST b) (cf p (SND b)) env) branches)
+         env) /\
   cf _ _ = cf_bottom`
 
   (WF_REL_TAC `measure (exp_size o SND)` \\ rw []
@@ -645,6 +1174,10 @@ val cf_def = tDefine "cf" `
        every_case_tac \\ fs [astTheory.exp_size_def] \\
        drule Fun_body_exp_size \\ strip_tac \\ fs [astTheory.exp_size_def]
      )
+     THEN1 (
+       Induct_on `branches` \\ fs [MEM] \\ rpt strip_tac \\ rw [] \\
+       fs [astTheory.exp_size_def]
+     )
   )
 
 val cf_ind = fetch "-" "cf_ind"
@@ -652,7 +1185,7 @@ val cf_ind = fetch "-" "cf_ind"
 val cf_defs = [cf_def, cf_lit_def, cf_con_def, cf_var_def, cf_fundecl_def, cf_let_def,
                cf_opn_def, cf_opb_def, cf_aw8alloc_def, cf_aw8sub_def, cf_aw8length_def,
                cf_aw8update_def, cf_app_def, cf_ref_def, cf_assign_def, cf_deref_def,
-               cf_fundecl_rec_def, cf_bottom_def]
+               cf_fundecl_rec_def, cf_bottom_def, cf_mat_def]
 
 (*------------------------------------------------------------------*)
 (** Properties about [cf]. The main result is the proof of soundness,
@@ -766,15 +1299,15 @@ val app_of_sound_cf = Q.prove (
 
   Induct \\ rpt strip_tac \\ fs [naryClosure_def, LENGTH_CONS] \\ rw [] \\
   rename1 `extend_env (n::ns) (xv::xvs) _` \\ Cases_on `ns` \\
-  rfs [LENGTH_NIL, LENGTH_CONS, extend_env_def, naryFun_def, app_def]
-  THEN1 (irule app_basic_of_sound_cf \\ fs [do_opapp_def])
+  fs [LENGTH_NIL, LENGTH_CONS] \\ rw [] \\
+  rfs [extend_env_def, Once extend_env_v_def, naryFun_def, app_def]
+  THEN1 (irule app_basic_of_sound_cf \\ fs [extend_env_v_def, do_opapp_def])
   THEN1 (
-    rw [] \\ fs [] \\ rename1 `extend_env (n'::ns) (xv'::xvs) _` \\
+    rename1 `extend_env_v (n'::ns) (xv'::xvs) _` \\
     fs [app_basic_def] \\ rpt strip_tac \\ fs [do_opapp_def] \\
-    fs [SEP_EXISTS, cond_def, STAR_def, PULL_EXISTS] \\
+    fs [SEP_EXISTS, cond_def, STAR_def, PULL_EXISTS, SPLIT_emp2] \\
     fs [naryFun_def, naryClosure_def, Once bigStepTheory.evaluate_cases] \\
-    fs [SPLIT_emp2] \\ first_assum progress \\ instantiate \\
-    qexists_tac `{}` \\ SPLIT_TAC
+    first_assum progress \\ instantiate \\ qexists_tac `{}` \\ SPLIT_TAC
   )
 )
 
@@ -817,15 +1350,16 @@ val app_rec_of_sound_cf_aux = Q.prove (
   Cases_on `params` \\ rpt strip_tac \\ rw [] \\
   fs [LENGTH_CONS] \\ rfs [] \\ qpat_assum `xvs = _` (K all_tac) \\
   rename1 `extend_env_rec _ _ (n::params) (xv::xvs) _` \\
-  Cases_on `params` \\ rfs [LENGTH_NIL, LENGTH_CONS, extend_env_rec_def] \\
-  fs [extend_env_def, app_def]
+  Cases_on `params` \\ rfs [LENGTH_NIL, LENGTH_CONS] \\
+  fs [extend_env_rec_def, extend_env_v_rec_def] \\
+  fs [extend_env_def, extend_env_v_def, app_def]
   THEN1 (
     irule app_basic_of_sound_cf \\
     rpt_drule_then (fs o sing) do_opapp_naryRecclosure \\
     fs [naryFun_def, letrec_pull_params_names, build_rec_env_zip]
   )
   THEN1 (
-    rw [] \\ rename1 `extend_env (n'::params) (xv'::xvs) _` \\
+    rw [] \\ rename1 `extend_env_v (n'::params) (xv'::xvs) _` \\
     fs [app_basic_def] \\ rpt strip_tac \\
     rpt_drule_then (fs o sing) do_opapp_naryRecclosure \\
     fs [SEP_EXISTS, cond_def, STAR_def, PULL_EXISTS, SPLIT_emp2] \\
@@ -837,7 +1371,7 @@ val app_rec_of_sound_cf_aux = Q.prove (
         MAP (\ (f,_,_). naryRecclosure env (letrec_pull_params funs) f)
             (letrec_pull_params funs)) ++ env.v))
       (n'::params) body` \\ strip_tac
-    THEN1 (irule app_of_sound_cf \\ fs [])
+    THEN1 (irule app_of_sound_cf \\ fs [extend_env_def])
     THEN1 (
       fs [naryFun_def, naryClosure_def, Once bigStepTheory.evaluate_cases] \\
       fs [letrec_pull_params_cancel, letrec_pull_params_names] \\
@@ -901,6 +1435,7 @@ val cf_letrec_sound_aux = Q.prove (
     fs [fundecl_rec_aux_def] \\
     qpat_assum `_ = rest` (mp_tac o GSYM) \\ rw [] \\
     cf_strip_sound_full_tac \\ qpat_assum `sound _ e _` mp_tac \\
+    fs [extend_env_rec_def] \\
     fs [letrec_pull_params_names, extend_env_rec_build_rec_env] \\
     rewrite_tac [sound_def] \\ disch_then progress \\ instantiate
   )
@@ -999,6 +1534,61 @@ val cf_letrec_sound = Q.prove (
   rpt strip_tac \\ mp_tac (Q.SPECL [`funs`, `e`] cf_letrec_sound_aux) \\
   fs [] \\ disch_then (qspecl_then [`funs`, `[]`] mp_tac) \\
   fs [letrec_pull_params_names, letrec_pull_params_def]
+)
+
+val PMATCH_EVAL_PMATCH_ROW_of_pat =
+  let
+    val pmatch_row_tm =
+        concl PMATCH_EVAL |> rand |> lhs |> rand |> rator |> rand
+    val pmatch_row_of_pat_tm =
+        PMATCH_ROW_of_pat_def |> SPEC_ALL |> concl |> rhs
+    val (tmsubst, tysubst) = match_term pmatch_row_tm pmatch_row_of_pat_tm
+    val thm = PMATCH_EVAL |> INST_TYPE tysubst |> INST tmsubst
+  in
+    SPEC_ALL (REWRITE_RULE [GSYM PMATCH_ROW_of_pat_def] thm)
+  end
+
+val PMATCH_evaluate_match = store_thm ("PMATCH_evaluate_match",
+  ``!v env H Q pats exps cfs branch_cf p exp st h_i h_k bind_exn_v.
+      LENGTH pats = LENGTH exps ==>
+      LENGTH exps = LENGTH cfs ==>
+      (!s. EVERY (\pat. validate_pat env.c s pat v env.v) pats) ==>
+      PMATCH (SOME v) (MAP2 (\pat cf. PMATCH_ROW_of_pat pat cf env) pats cfs) = branch_cf ==>
+      branch_cf <> PMATCH_INCOMPLETE ==>
+      branch_cf env H Q ==>
+      EVERY2 (\exp cf. sound p exp cf) exps cfs ==>
+      SPLIT (st2heap p st) (h_i, h_k) ==> H h_i ==>
+      ?v' st' h_f h_g.
+        bigStep$evaluate_match F env st v (ZIP (pats, exps)) bind_exn_v (st', Rval v') /\
+        Q v' h_f /\ SPLIT3 (st2heap p st') (h_f, h_k, h_g)``,
+  Induct_on `pats` \\ fs [] \\ rpt strip_tac
+  THEN1 (
+    rpt (qpat_assum `0 = LENGTH _` (assume_tac o GSYM) \\ fs [LENGTH_NIL]) \\ rw [] \\
+    fs [PMATCH_def]
+  ) \\
+
+  fs [LENGTH_CONS] \\ rename1 `exps = exp::exps'` \\ rw [] \\
+  fs [LENGTH_CONS] \\ rename1 `cfs = exp_cf::cfs'` \\ rw [] \\ fs [] \\
+  rename1 `PMATCH_ROW_of_pat pat _ _` \\
+  fs [PMATCH_def, option_case_compute] \\ full_case_tac
+  THEN1 (
+    first_assum (qspec_then `st.refs` strip_assume_tac) \\
+    fs [validate_pat_def, IS_SOME_EXISTS] \\ fs [THE_DEF] \\
+    fs [Once bigStepTheory.evaluate_cases] \\
+    rpt_drule_then (qspec_then `st.refs` strip_assume_tac) PMATCH_ROW_pmatch \\
+    fs [] \\ qpat_assum `sound _ _ exp_cf` (progress o REWRITE_RULE [sound_def]) \\
+    instantiate
+  )
+  THEN1 (
+    fs [NOT_IS_SOME_EQ_NONE] \\
+    first_assum (qspec_then `st.refs` assume_tac) \\
+    fs [validate_pat_def, pat_typechecks_def] \\
+    mp_tac (fst (CONJ_PAIR PMATCH_ROW_pmatch_nomatch)
+            |> INST_TYPE [alpha |-> ``:hprop -> (v -> hprop) -> bool``]) \\ (* ? *)
+    disch_then progress \\
+    once_rewrite_tac [bigStepTheory.evaluate_cases] \\ fs [] \\
+    first_assum irule \\ fs [] \\ instantiate
+  )
 )
 
 val cf_sound = store_thm ("cf_sound",
@@ -1244,6 +1834,26 @@ val cf_sound = store_thm ("cf_sound",
       qexists_tac `{}` \\ mp_tac store2heap_IN_unique_key \\ rpt strip_tac
       THEN1 (first_assum irule \\ instantiate \\ SPLIT_TAC)
       THEN1 (rpt_drule_then (fs o sing) store2heap_LUPDATE \\ SPLIT_TAC)
+    )
+  )
+  THEN1 (
+    (* Mat *)
+    cf_strip_sound_full_tac \\
+    `evaluate F env st e (st, Rval v)` by (fs [exp2v_evaluate]) \\
+    instantiate \\
+    `branches = ZIP (MAP FST branches, MAP SND branches)`
+      by (fs [GSYM UNZIP_MAP, ZIP_UNZIP]) \\ pop_assum (fs o sing o Once) \\
+    fs [GSYM CONJ_ASSOC] \\ irule PMATCH_evaluate_match \\ fs [MAP_ZIP] \\
+    GEN_EXISTS_TAC "cfs" `MAP (\b. cf p (SND b)) branches` \\
+    fs [MAP2_ZIP] \\ instantiate \\ rpt strip_tac \\
+    try_finally (
+      Induct_on `branches` \\ fs [] \\ rpt strip_tac \\
+      fs [PMATCH_EVAL_PMATCH_ROW_of_pat] \\ every_case_tac \\ fs []
+    )
+    THEN1 (
+      fs [LIST_REL_EVERY_ZIP] \\ fs [EVERY_MEM, MEM_ZIP] \\ rpt strip_tac \\
+      rename1 `_ exp_cf_pair` \\ Cases_on `exp_cf_pair` \\
+      fs [EL_MAP] \\ first_assum irule \\ instantiate \\ fs [EL_MAP]
     )
   )
 )
